Add nth_odd and prove basic facts about it

ETCS_Parity.thy
@@ -78,6 +78,83 @@ proof (rule natural_number_object_func_unique[where f="successor \<circ>\<^sub>c
   qed
 qed
 
+definition nth_odd :: "cfunc" where
+  "nth_odd = (THE u. u: \<nat>\<^sub>c \<rightarrow> \<nat>\<^sub>c \<and> 
+    u \<circ>\<^sub>c zero = successor \<circ>\<^sub>c zero \<and>
+    (successor \<circ>\<^sub>c successor) \<circ>\<^sub>c u = u \<circ>\<^sub>c successor)"
+
+lemma nth_odd_def2:
+  "nth_odd: \<nat>\<^sub>c \<rightarrow> \<nat>\<^sub>c \<and> nth_odd \<circ>\<^sub>c zero = successor \<circ>\<^sub>c zero \<and> (successor \<circ>\<^sub>c successor) \<circ>\<^sub>c nth_odd = nth_odd \<circ>\<^sub>c successor"
+  by (unfold nth_odd_def, rule theI', typecheck_cfuncs, rule natural_number_object_property2, auto)
+
+lemma nth_odd_type[type_rule]:
+  "nth_odd: \<nat>\<^sub>c \<rightarrow> \<nat>\<^sub>c"
+  by (simp add: nth_odd_def2)
+
+lemma nth_odd_zero:
+  "nth_odd \<circ>\<^sub>c zero = successor \<circ>\<^sub>c zero"
+  by (simp add: nth_odd_def2)
+
+lemma nth_odd_successor:
+  "nth_odd \<circ>\<^sub>c successor = (successor \<circ>\<^sub>c successor) \<circ>\<^sub>c nth_odd"
+  by (simp add: nth_odd_def2)
+
+lemma nth_odd_successor2:
+  "nth_odd \<circ>\<^sub>c successor = successor \<circ>\<^sub>c successor \<circ>\<^sub>c nth_odd"
+  using comp_associative2 nth_odd_def2 by (typecheck_cfuncs, auto)
+
+lemma nth_odd_is_succ_times_two:
+  "nth_odd = successor \<circ>\<^sub>c mult2 \<circ>\<^sub>c \<langle>(successor \<circ>\<^sub>c successor \<circ>\<^sub>c zero) \<circ>\<^sub>c \<beta>\<^bsub>\<nat>\<^sub>c\<^esub>, id \<nat>\<^sub>c\<rangle>"
+proof (rule natural_number_object_func_unique[where f="successor \<circ>\<^sub>c successor", where X="\<nat>\<^sub>c"])
+  show "nth_odd : \<nat>\<^sub>c \<rightarrow> \<nat>\<^sub>c"
+    by typecheck_cfuncs
+  show "successor \<circ>\<^sub>c mult2 \<circ>\<^sub>c \<langle>(successor \<circ>\<^sub>c successor \<circ>\<^sub>c zero) \<circ>\<^sub>c \<beta>\<^bsub>\<nat>\<^sub>c\<^esub>, id \<nat>\<^sub>c\<rangle> : \<nat>\<^sub>c \<rightarrow> \<nat>\<^sub>c"
+    by typecheck_cfuncs
+  show "successor \<circ>\<^sub>c successor : \<nat>\<^sub>c \<rightarrow> \<nat>\<^sub>c"
+    by typecheck_cfuncs
+
+  show "nth_odd \<circ>\<^sub>c zero =
+    (successor \<circ>\<^sub>c mult2 \<circ>\<^sub>c \<langle>(successor \<circ>\<^sub>c successor \<circ>\<^sub>c zero) \<circ>\<^sub>c \<beta>\<^bsub>\<nat>\<^sub>c\<^esub>,id\<^sub>c \<nat>\<^sub>c\<rangle>) \<circ>\<^sub>c zero"
+  proof -
+    have "(successor \<circ>\<^sub>c mult2 \<circ>\<^sub>c \<langle>(successor \<circ>\<^sub>c successor \<circ>\<^sub>c zero) \<circ>\<^sub>c \<beta>\<^bsub>\<nat>\<^sub>c\<^esub>,id\<^sub>c \<nat>\<^sub>c\<rangle>) \<circ>\<^sub>c zero
+      = successor \<circ>\<^sub>c mult2 \<circ>\<^sub>c \<langle>(successor \<circ>\<^sub>c successor \<circ>\<^sub>c zero) \<circ>\<^sub>c \<beta>\<^bsub>\<nat>\<^sub>c\<^esub>,id\<^sub>c \<nat>\<^sub>c\<rangle> \<circ>\<^sub>c zero"
+      by (typecheck_cfuncs, simp add: comp_associative2)
+    also have "... = successor \<circ>\<^sub>c mult2 \<circ>\<^sub>c \<langle>successor \<circ>\<^sub>c successor \<circ>\<^sub>c zero, zero\<rangle>"
+      by (typecheck_cfuncs, simp add: cart_prod_extract_right)
+    also have "... = successor \<circ>\<^sub>c zero"
+      using mult_def mult_respects_zero_right succ_n_type zero_type by auto
+    also have "... = nth_odd \<circ>\<^sub>c zero"
+      by (simp add: nth_odd_def2)
+    then show ?thesis
+      using calculation by auto
+  qed
+
+  show "nth_odd \<circ>\<^sub>c successor = (successor \<circ>\<^sub>c successor) \<circ>\<^sub>c nth_odd"
+    by (simp add: nth_odd_successor)
+
+  show "(successor \<circ>\<^sub>c mult2 \<circ>\<^sub>c \<langle>(successor \<circ>\<^sub>c successor \<circ>\<^sub>c zero) \<circ>\<^sub>c \<beta>\<^bsub>\<nat>\<^sub>c\<^esub>,id\<^sub>c \<nat>\<^sub>c\<rangle>) \<circ>\<^sub>c successor =
+    (successor \<circ>\<^sub>c successor) \<circ>\<^sub>c  successor \<circ>\<^sub>c mult2 \<circ>\<^sub>c \<langle>(successor \<circ>\<^sub>c successor \<circ>\<^sub>c zero) \<circ>\<^sub>c \<beta>\<^bsub>\<nat>\<^sub>c\<^esub>,id\<^sub>c \<nat>\<^sub>c\<rangle>"
+  proof -
+    have "(successor \<circ>\<^sub>c mult2 \<circ>\<^sub>c \<langle>(successor \<circ>\<^sub>c successor \<circ>\<^sub>c zero) \<circ>\<^sub>c \<beta>\<^bsub>\<nat>\<^sub>c\<^esub>,id\<^sub>c \<nat>\<^sub>c\<rangle>) \<circ>\<^sub>c successor
+      = successor \<circ>\<^sub>c mult2 \<circ>\<^sub>c \<langle>(successor \<circ>\<^sub>c successor \<circ>\<^sub>c zero) \<circ>\<^sub>c \<beta>\<^bsub>\<nat>\<^sub>c\<^esub>,id\<^sub>c \<nat>\<^sub>c\<rangle> \<circ>\<^sub>c successor"
+      by (typecheck_cfuncs, simp add: comp_associative2)
+    also have "... = successor \<circ>\<^sub>c mult2 \<circ>\<^sub>c \<langle>(successor \<circ>\<^sub>c successor \<circ>\<^sub>c zero) \<circ>\<^sub>c \<beta>\<^bsub>\<nat>\<^sub>c\<^esub>, successor\<rangle>"
+      by (typecheck_cfuncs, smt cfunc_prod_comp comp_associative2 id_left_unit2 terminal_func_comp)
+    also have "... = successor \<circ>\<^sub>c add2 \<circ>\<^sub>c \<langle>(successor \<circ>\<^sub>c successor \<circ>\<^sub>c zero) \<circ>\<^sub>c  \<beta>\<^bsub>\<nat>\<^sub>c\<^esub>,mult2 \<circ>\<^sub>c \<langle>(successor \<circ>\<^sub>c successor \<circ>\<^sub>c zero) \<circ>\<^sub>c \<beta>\<^bsub>\<nat>\<^sub>c\<^esub>,id\<^sub>c \<nat>\<^sub>c\<rangle>\<rangle>"
+      using mult2_respects_succ_right by (typecheck_cfuncs, auto)
+    also have "... = successor \<circ>\<^sub>c add2 \<circ>\<^sub>c \<langle>successor \<circ>\<^sub>c successor \<circ>\<^sub>c zero \<circ>\<^sub>c  \<beta>\<^bsub>\<nat>\<^sub>c\<^esub>,mult2 \<circ>\<^sub>c \<langle>(successor \<circ>\<^sub>c successor \<circ>\<^sub>c zero) \<circ>\<^sub>c \<beta>\<^bsub>\<nat>\<^sub>c\<^esub>,id\<^sub>c \<nat>\<^sub>c\<rangle>\<rangle>"
+      by (typecheck_cfuncs, simp add: comp_associative2)
+    also have "... = successor \<circ>\<^sub>c successor \<circ>\<^sub>c successor \<circ>\<^sub>c add2 \<circ>\<^sub>c \<langle>zero \<circ>\<^sub>c  \<beta>\<^bsub>\<nat>\<^sub>c\<^esub>,mult2 \<circ>\<^sub>c \<langle>(successor \<circ>\<^sub>c successor \<circ>\<^sub>c zero) \<circ>\<^sub>c \<beta>\<^bsub>\<nat>\<^sub>c\<^esub>,id\<^sub>c \<nat>\<^sub>c\<rangle>\<rangle>"
+      by (typecheck_cfuncs, simp add: add2_commutes_succ add2_respects_succ_right)
+    also have "... = successor \<circ>\<^sub>c successor \<circ>\<^sub>c successor \<circ>\<^sub>c mult2 \<circ>\<^sub>c \<langle>(successor \<circ>\<^sub>c successor \<circ>\<^sub>c zero) \<circ>\<^sub>c \<beta>\<^bsub>\<nat>\<^sub>c\<^esub>,id\<^sub>c \<nat>\<^sub>c\<rangle>"
+      by (typecheck_cfuncs, simp add: add2_respects_zero_on_left)
+    also have "... = (successor \<circ>\<^sub>c successor) \<circ>\<^sub>c successor \<circ>\<^sub>c mult2 \<circ>\<^sub>c \<langle>(successor \<circ>\<^sub>c successor \<circ>\<^sub>c zero) \<circ>\<^sub>c \<beta>\<^bsub>\<nat>\<^sub>c\<^esub>,id\<^sub>c \<nat>\<^sub>c\<rangle>"
+      by (typecheck_cfuncs, smt comp_associative2)
+    then show ?thesis
+      using calculation by auto
+  qed
+qed
+
 (*lemma odd_even_iso:
   "isomorphism (
     (successor \<circ>\<^sub>c mult2 \<circ>\<^sub>c \<langle>(successor \<circ>\<^sub>c successor \<circ>\<^sub>c zero) \<circ>\<^sub>c \<beta>\<^bsub>\<nat>\<^sub>c\<^esub>, id \<nat>\<^sub>c\<rangle>)
